coq/bls.v
@@ -1,0 +1,665 @@
+Require Import Lib.
+Require Import IntTypes.
+From Coq Require Import ZArith.
+Require Import List. Import ListNotations.
+Open Scope hacspec_scope.
+Open Scope bool_scope.
+
+Notation "a >?? b" := (Nat.ltb b a) (at level 79).
+
+(* uint_size = nat *)
+
+
+Module Wordsize_0x1a0111ea397fe69a4b1ba7b6434bacd764774b84f38512bf6730d2a0f6b0f6241eabfffeb153ffffb9feffffffffaaab.
+  Definition wordsize : nat := 0x1a0111ea397fe69a4b1ba7b6434bacd764774b84f38512bf6730d2a0f6b0f6241eabfffeb153ffffb9feffffffffaaab.
+  Remark wordsize_not_zero: wordsize <> 0%nat.
+  Proof. Admitted.
+  (* Proof. unfold wordsize; congruence. Qed. *)
+End Wordsize_0x1a0111ea397fe69a4b1ba7b6434bacd764774b84f38512bf6730d2a0f6b0f6241eabfffeb153ffffb9feffffffffaaab.
+Strategy opaque [Wordsize_0x1a0111ea397fe69a4b1ba7b6434bacd764774b84f38512bf6730d2a0f6b0f6241eabfffeb153ffffb9feffffffffaaab.wordsize].
+
+Module nat_mod_0x1a0111ea397fe69a4b1ba7b6434bacd764774b84f38512bf6730d2a0f6b0f6241eabfffeb153ffffb9feffffffffaaab := Integers.Make(Wordsize_0x1a0111ea397fe69a4b1ba7b6434bacd764774b84f38512bf6730d2a0f6b0f6241eabfffeb153ffffb9feffffffffaaab).
+Import nat_mod_0x1a0111ea397fe69a4b1ba7b6434bacd764774b84f38512bf6730d2a0f6b0f6241eabfffeb153ffffb9feffffffffaaab.
+
+Definition fp : Type :=
+  nat_mod_0x1a0111ea397fe69a4b1ba7b6434bacd764774b84f38512bf6730d2a0f6b0f6241eabfffeb153ffffb9feffffffffaaab.int.
+
+
+Definition g1 : Type := (fp * fp * bool).
+Definition fp2 : Type := (fp * fp).
+Definition g2 : Type := (fp2 * fp2 * bool).
+Definition fp6 : Type := (fp2 * fp2 * fp2).
+Definition fp12 : Type := (fp6 * fp6).
+
+Definition fp_canvas := lseq (pub_uint8) (48).
+
+
+Definition serialized_fp := lseq (uint8) (usize 48).
+
+Definition array_fp := lseq (uint64) (usize 6).
+
+Definition scalar_canvas := lseq (pub_uint8) (32).
+
+Module Wordsize_0x8000000000000000000000000000000000000000000000000000000000000000.
+  Definition wordsize : nat := 0x8000000000000000000000000000000000000000000000000000000000000000.
+  Remark wordsize_not_zero: wordsize <> 0%nat.
+  Proof. Admitted.
+  (* Proof. unfold wordsize; congruence. Qed. *)
+End Wordsize_0x8000000000000000000000000000000000000000000000000000000000000000.
+Strategy opaque [Wordsize_0x8000000000000000000000000000000000000000000000000000000000000000.wordsize].
+
+Module nat_mod_0x8000000000000000000000000000000000000000000000000000000000000000 := Integers.Make(Wordsize_0x8000000000000000000000000000000000000000000000000000000000000000).
+(* Import nat_mod_0x8000000000000000000000000000000000000000000000000000000000000000. *)
+
+Definition scalar :=
+  nat_mod_0x8000000000000000000000000000000000000000000000000000000000000000.int.
+
+(* TODO *)
+Axiom nat_bit : N -> scalar -> uint_size -> bool.
+Axiom most_significant_bit : scalar -> uint_size -> uint_size.
+Axiom N_to_int : N -> int.
+Coercion N_to_int : N >-> int.
+Coercion Z.of_N : N >-> Z.
+
+(* TODO: write a coq-friendly version of this (coq can't find decreasing fix of the body) *)
+(* Fixpoint most_significant_bit (m_0 : scalar) (n_1 : uint_size) : uint_size :=
+  if (
+    ((n_1) >?? (usize 0)) && (
+      negb (
+        nat_bit (
+          0x8000000000000000000000000000000000000000000000000000000000000000) (
+          m_0) (n_1)))) then (
+    most_significant_bit (m_0) ((n_1) - (usize 1))) else (n_1). *)
+
+Definition nat_zero := zero.
+Definition nat_one := one.
+Definition nat_two := repr 2.
+(* compcert doesn't have modular multiplicative inverse for some reason? *)
+Axiom nat_inv : int -> int.
+Axiom nat_inv_is_multiplicative_inverse : forall (n : int), mul n (nat_inv n) = one.  
+
+
+Definition nat_exp (x y : int) := repr (Z.pow (unsigned x) (unsigned y)).
+
+
+Definition fp2fromfp (n_2 : fp) : fp2 :=
+(
+  n_2,
+  zero
+).
+
+Definition fp2zero : fp2 :=
+  fp2fromfp (
+    nat_zero).
+
+Infix "-" := sub.
+Infix "+" := add.
+Infix "*" := mul.
+
+Definition fp2neg (n_3 : fp2) : fp2 :=
+  let (n1_4, n2_5) := n_3 in
+  (
+    (
+      nat_zero) - (
+      n1_4),
+    (
+      nat_zero) - (
+      n2_5)
+  ).
+
+Definition fp2add (n_6 : fp2) (m_7 : fp2) : fp2 :=
+  let (n1_8, n2_9) := n_6 in
+  let (m1_10, m2_11) := m_7 in
+  ((n1_8) + (m1_10), (n2_9) + (m2_11)).
+
+Definition fp2sub (n_12 : fp2) (m_13 : fp2) : fp2 :=
+  fp2add (n_12) (fp2neg (m_13)).
+
+Definition fp2mul (n_14 : fp2) (m_15 : fp2) : fp2 :=
+  let (n1_16, n2_17) := n_14 in
+  let (m1_18, m2_19) := m_15 in
+  let x1_20 := ((n1_16) * (m1_18)) - ((n2_17) * (m2_19)) in
+  let x2_21 := ((n1_16) * (m2_19)) + ((n2_17) * (m1_18)) in
+  (x1_20, x2_21).
+
+
+Definition fp2inv (n_22 : fp2) : fp2 :=
+  let (n1_23, n2_24) := n_22 in
+  let t0_25 := ((n1_23) * (n1_23)) + ((n2_24) * (n2_24)) in
+  let t1_26 :=
+    nat_inv (
+      t0_25)
+  in
+  let x1_27 := (n1_23) * (t1_26) in
+  let x2_28 :=
+    (
+      nat_zero) - (
+      (n2_24) * (t1_26))
+  in
+  (x1_27, x2_28).
+
+Definition fp2conjugate (n_29 : fp2) : fp2 :=
+  let (n1_30, n2_31) := n_29 in
+  (
+    n1_30,
+    (
+      nat_zero) - (
+      n2_31)
+  ).
+
+Definition fp6fromfp2 (n_32 : fp2) : fp6 :=
+  (n_32, fp2zero, fp2zero).
+
+Definition fp6zero : fp6 :=
+  fp6fromfp2 (fp2zero).
+
+Definition fp6neg (n_33 : fp6) : fp6 :=
+  let '(n1_34, n2_35, n3_36) := n_33 in
+  (
+    fp2sub (fp2zero) (n1_34),
+    fp2sub (fp2zero) (n2_35),
+    fp2sub (fp2zero) (n3_36)
+  ).
+
+Definition fp6add (n_37 : fp6) (m_38 : fp6) : fp6 :=
+  let '(n1_39, n2_40, n3_41) := n_37 in
+  let '(m1_42, m2_43, m3_44) := m_38 in
+  (fp2add (n1_39) (m1_42), fp2add (n2_40) (m2_43), fp2add (n3_41) (m3_44)).
+
+Definition fp6sub (n_45 : fp6) (m_46 : fp6) : fp6 :=
+  fp6add (n_45) (fp6neg (m_46)).
+
+Definition fp6mul (n_47 : fp6) (m_48 : fp6) : fp6 :=
+  let '(n1_49, n2_50, n3_51) := n_47 in
+  let '(m1_52, m2_53, m3_54) := m_48 in
+  let eps_55 :=
+    (
+      nat_one,
+      nat_one
+    )
+  in
+  let t1_56 := fp2mul (n1_49) (m1_52) in
+  let t2_57 := fp2mul (n2_50) (m2_53) in
+  let t3_58 := fp2mul (n3_51) (m3_54) in
+  let t4_59 := fp2mul (fp2add (n2_50) (n3_51)) (fp2add (m2_53) (m3_54)) in
+  let t5_60 := fp2sub (fp2sub (t4_59) (t2_57)) (t3_58) in
+  let x_61 := fp2add (fp2mul (t5_60) (eps_55)) (t1_56) in
+  let t4_62 := fp2mul (fp2add (n1_49) (n2_50)) (fp2add (m1_52) (m2_53)) in
+  let t5_63 := fp2sub (fp2sub (t4_62) (t1_56)) (t2_57) in
+  let y_64 := fp2add (t5_63) (fp2mul (eps_55) (t3_58)) in
+  let t4_65 := fp2mul (fp2add (n1_49) (n3_51)) (fp2add (m1_52) (m3_54)) in
+  let t5_66 := fp2sub (fp2sub (t4_65) (t1_56)) (t3_58) in
+  let z_67 := fp2add (t5_66) (t2_57) in
+  (x_61, y_64, z_67).
+
+Definition fp6inv (n_68 : fp6) : fp6 :=
+  let '(n1_69, n2_70, n3_71) := n_68 in
+  let eps_72 :=
+    (
+      nat_one,
+      nat_one
+    )
+  in
+  let t1_73 := fp2mul (n1_69) (n1_69) in
+  let t2_74 := fp2mul (n2_70) (n2_70) in
+  let t3_75 := fp2mul (n3_71) (n3_71) in
+  let t4_76 := fp2mul (n1_69) (n2_70) in
+  let t5_77 := fp2mul (n1_69) (n3_71) in
+  let t6_78 := fp2mul (n2_70) (n3_71) in
+  let x0_79 := fp2sub (t1_73) (fp2mul (eps_72) (t6_78)) in
+  let y0_80 := fp2sub (fp2mul (eps_72) (t3_75)) (t4_76) in
+  let z0_81 := fp2sub (t2_74) (t5_77) in
+  let t0_82 := fp2mul (n1_69) (x0_79) in
+  let t0_83 := fp2add (t0_82) (fp2mul (eps_72) (fp2mul (n3_71) (y0_80))) in
+  let t0_84 := fp2add (t0_83) (fp2mul (eps_72) (fp2mul (n2_70) (z0_81))) in
+  let t0_85 := fp2inv (t0_84) in
+  let x_86 := fp2mul (x0_79) (t0_85) in
+  let y_87 := fp2mul (y0_80) (t0_85) in
+  let z_88 := fp2mul (z0_81) (t0_85) in
+  (x_86, y_87, z_88).
+
+Definition fp12fromfp6 (n_89 : fp6) : fp12 :=
+  (n_89, fp6zero).
+
+Definition fp12neg (n_90 : fp12) : fp12 :=
+  let '(n1_91, n2_92) := n_90 in
+  (fp6sub (fp6zero ) (n1_91), fp6sub (fp6zero ) (n2_92)).
+
+Definition fp12add (n_93 : fp12) (m_94 : fp12) : fp12 :=
+  let '(n1_95, n2_96) := n_93 in
+  let '(m1_97, m2_98) := m_94 in
+  (fp6add (n1_95) (m1_97), fp6add (n2_96) (m2_98)).
+
+Definition fp12sub (n_99 : fp12) (m_100 : fp12) : fp12 :=
+  fp12add (n_99) (fp12neg (m_100)).
+
+Definition fp12mul (n_101 : fp12) (m_102 : fp12) : fp12 :=
+  let '(n1_103, n2_104) := n_101 in
+  let '(m1_105, m2_106) := m_102 in
+  let gamma_107 :=
+    (
+      fp2zero,
+      fp2fromfp (
+        nat_one),
+      fp2zero
+    )
+  in
+  let t1_108 := fp6mul (n1_103) (m1_105) in
+  let t2_109 := fp6mul (n2_104) (m2_106) in
+  let x_110 := fp6add (t1_108) (fp6mul (t2_109) (gamma_107)) in
+  let y_111 := fp6mul (fp6add (n1_103) (n2_104)) (fp6add (m1_105) (m2_106)) in
+  let y_112 := fp6sub (fp6sub (y_111) (t1_108)) (t2_109) in
+  (x_110, y_112).
+
+Definition fp12inv (n_113 : fp12) : fp12 :=
+  let '(n1_114, n2_115) := n_113 in
+  let gamma_116 :=
+    (
+      fp2zero,
+      fp2fromfp (
+        nat_one),
+      fp2zero
+    )
+  in
+  let t1_117 := fp6mul (n1_114) (n1_114) in
+  let t2_118 := fp6mul (n2_115) (n2_115) in
+  let t1_119 := fp6sub (t1_117) (fp6mul (gamma_116) (t2_118)) in
+  let t2_120 := fp6inv (t1_119) in
+  let x_121 := fp6mul (n1_114) (t2_120) in
+  let y_122 := fp6neg (fp6mul (n2_115) (t2_120)) in
+  (x_121, y_122).
+
+Definition int_to_nat (n : int) : nat := unsigned n.
+
+Coercion int_to_nat : int >-> nat.
+
+Definition fp12exp (n_123 : fp12) (k_124 : scalar) : fp12 :=
+  let l_125 := (usize 255) - (most_significant_bit (k_124) (usize 255)) in
+  let c_126 := n_123 in
+  let '(c_126) :=
+    foldi (l_125) (usize 255) (fun i_127 c_126 =>
+      let c_126 := fp12mul (c_126) (c_126) in
+      let '(c_126) :=
+        if nat_bit (
+          0x8000000000000000000000000000000000000000000000000000000000000000) (
+          k_124) (((usize 255) - (i_127)) - (usize 1)) then (
+          let c_126 := fp12mul (c_126) (n_123) in
+          (c_126)
+        ) else ( (c_126)
+        )
+      in
+      (c_126))
+    (c_126)
+  in
+  c_126.
+
+Definition fp12conjugate (n_128 : fp12) : fp12 :=
+  let '(n1_129, n2_130) := n_128 in
+  (n1_129, fp6neg (n2_130)).
+
+Definition fp12zero  : fp12 :=
+  fp12fromfp6 (fp6zero ).
+
+Definition g1add_a (p_131 : g1) (q_132 : g1) : g1 :=
+  let '(x1_133, y1_134, _) := p_131 in
+  let '(x2_135, y2_136, _) := q_132 in
+  let x_diff_137 := (x2_135) - (x1_133) in
+  let y_diff_138 := (y2_136) - (y1_134) in
+  let xovery_139 :=
+    (y_diff_138) * (
+      nat_inv (
+        x_diff_137))
+  in
+  let x3_140 :=
+    (
+      (
+        nat_exp (
+          xovery_139) (pub_u32 2)) - (x1_133)) - (x2_135)
+  in
+  let y3_141 := ((xovery_139) * ((x1_133) - (x3_140))) - (y1_134) in
+  (x3_140, y3_141, false).
+
+Definition g1double_a (p_142 : g1) : g1 :=
+  let '(x1_143, y1_144, _) := p_142 in
+  let x12_145 :=
+    nat_exp (
+      x1_143) (pub_u32 2)
+  in
+  let xovery_146 :=
+    ((repr (pub_u128 3)) * (x12_145)) * (
+      nat_inv ((nat_two  * (y1_144)))) in
+  let x3_147 :=
+    (
+      nat_exp (
+        xovery_146) (pub_u32 2)) - (
+      (
+        nat_two  * (
+        x1_143)))
+  in
+  let y3_148 := ((xovery_146) * ((x1_143) - (x3_147))) - (y1_144) in
+  (x3_147, y3_148, false).
+
+(* TODO *)
+Axiom g1_eqb : g1 -> g1 -> bool.
+
+Definition g1add (p_149 : g1) (q_150 : g1) : g1 :=
+  let '(x1_151, y1_152, inf1_153) := p_149 in
+  let '(x2_154, y2_155, inf2_156) := q_150 in
+  if (inf1_153) then (q_150) else (
+    if (inf2_156) then (p_149) else (
+      if (g1_eqb (p_149) (q_150)) then (g1double_a (p_149)) else (
+        if (
+          negb (
+            (eq (x1_151) (x2_154)) && (
+              eq (y1_152)  (
+                (
+                  nat_zero) - (
+                  y2_155))))) then (g1add_a (p_149) (q_150)) else (
+          (
+            nat_zero,
+            nat_zero,
+            true
+          ))))).
+
+Definition g1double (p_157 : g1) : g1 :=
+  let '(x1_158, y1_159, inf1_160) := p_157 in
+  if (
+    (negb (eq
+       (y1_159) (
+        nat_zero))) && (
+      negb (inf1_160))) then (g1double_a (p_157)) else (
+    (
+      nat_zero,
+      nat_zero,
+      true
+    )).
+
+Definition g1mul (m_161 : scalar) (p_162 : g1) : g1 :=
+  let n_163 := usize 255 in
+  let k_164 := (n_163) - (most_significant_bit (m_161) (n_163)) in
+  let t_165 := p_162 in
+  let '(t_165) :=
+    foldi (k_164) (n_163) (fun i_166 t_165 =>
+      let t_165 := g1double (t_165) in
+      let '(t_165) :=
+        if nat_bit (
+          0x8000000000000000000000000000000000000000000000000000000000000000) (
+          m_161) (((n_163) - (i_166)) - (usize 1)) then (
+          let t_165 := g1add (t_165) (p_162) in
+          (t_165)
+        ) else ( (t_165)
+        )
+      in
+      (t_165))
+    (t_165)
+  in
+  t_165.
+
+Definition g1neg (p_167 : g1) : g1 :=
+  let '(x_168, y_169, inf_170) := p_167 in
+  (
+    x_168,
+    (
+      nat_zero) - (
+      y_169),
+    inf_170
+  ).
+
+Definition g2add_a (p_171 : g2) (q_172 : g2) : g2 :=
+  let '(x1_173, y1_174, _) := p_171 in
+  let '(x2_175, y2_176, _) := q_172 in
+  let x_diff_177 := fp2sub (x2_175) (x1_173) in
+  let y_diff_178 := fp2sub (y2_176) (y1_174) in
+  let xovery_179 := fp2mul (y_diff_178) (fp2inv (x_diff_177)) in
+  let t1_180 := fp2mul (xovery_179) (xovery_179) in
+  let t2_181 := fp2sub (t1_180) (x1_173) in
+  let x3_182 := fp2sub (t2_181) (x2_175) in
+  let t1_183 := fp2sub (x1_173) (x3_182) in
+  let t2_184 := fp2mul (xovery_179) (t1_183) in
+  let y3_185 := fp2sub (t2_184) (y1_174) in
+  (x3_182, y3_185, false).
+
+Definition g2double_a (p_186 : g2) : g2 :=
+  let '(x1_187, y1_188, _) := p_186 in
+  let x12_189 := fp2mul (x1_187) (x1_187) in
+  let t1_190 :=
+    fp2mul (
+      fp2fromfp (
+        repr (
+          pub_u128 3))) (x12_189)
+  in
+  let t2_191 :=
+    fp2inv (
+      fp2mul (
+        fp2fromfp nat_two) (y1_188))
+  in
+  let xovery_192 := fp2mul (t1_190) (t2_191) in
+  let t1_193 := fp2mul (xovery_192) (xovery_192) in
+  let t2_194 :=
+    fp2mul (
+      fp2fromfp (
+        nat_two )) (
+      x1_187)
+  in
+  let x3_195 := fp2sub (t1_193) (t2_194) in
+  let t1_196 := fp2sub (x1_187) (x3_195) in
+  let t2_197 := fp2mul (xovery_192) (t1_196) in
+  let y3_198 := fp2sub (t2_197) (y1_188) in
+  (x3_195, y3_198, false).
+
+(* TODO *)
+Axiom g2_eqb : g2 -> g2 -> bool.
+Axiom fp2_eqb : fp2 -> fp2 -> bool.
+
+Definition g2add (p_199 : g2) (q_200 : g2) : g2 :=
+  let '(x1_201, y1_202, inf1_203) := p_199 in
+  let '(x2_204, y2_205, inf2_206) := q_200 in
+  if (inf1_203) then (q_200) else (
+    if (inf2_206) then (p_199) else (
+      if (g2_eqb (p_199) (q_200)) then (g2double_a (p_199)) else (
+        if (
+          negb (
+            (fp2_eqb (x1_201) (x2_204)) && (fp2_eqb (y1_202) (fp2neg (y2_205))))) then (
+          g2add_a (p_199) (q_200)) else ((fp2zero, fp2zero, true))))).
+
+Definition g2double (p_207 : g2) : g2 :=
+  let '(x1_208, y1_209, inf1_210) := p_207 in
+  if ((fp2_eqb (y1_209)  (fp2zero)) && (negb (inf1_210))) then (
+    g2double_a (p_207)) else ((fp2zero, fp2zero, true)).
+
+Definition g2mul (m_211 : scalar) (p_212 : g2) : g2 :=
+  let n_213 := usize 255 in
+  let k_214 := (n_213) - (most_significant_bit (m_211) (n_213)) in
+  let t_215 := p_212 in
+  let '(t_215) :=
+    foldi (k_214) (n_213) (fun i_216 t_215 =>
+      let t_215 := g2double (t_215) in
+      let '(t_215) :=
+        if nat_bit (
+          0x8000000000000000000000000000000000000000000000000000000000000000) (
+          m_211) (((n_213) - (i_216)) - (usize 1)) then (
+          let t_215 := g2add (t_215) (p_212) in
+          (t_215)
+        ) else ( (t_215)
+        )
+      in
+      (t_215))
+    (t_215)
+  in
+  t_215.
+
+Definition g2neg (p_217 : g2) : g2 :=
+  let '(x_218, y_219, inf_220) := p_217 in
+  (x_218, fp2neg (y_219), inf_220).
+
+Definition twist (p_221 : g1) : (fp12 * fp12) :=
+  let '(p0_222, p1_223, _) := p_221 in
+  let x_224 := ((fp2zero, fp2fromfp (p0_222), fp2zero), fp6zero ) in
+  let y_225 := (fp6zero , (fp2zero, fp2fromfp (p1_223), fp2zero)) in
+  (x_224, y_225).
+
+Definition line_double_p (r_226 : g2) (p_227 : g1) : fp12 :=
+  let '(r0_228, r1_229, _) := r_226 in
+  let a_230 :=
+    fp2mul (
+      fp2fromfp (
+        repr (
+          pub_u128 3))) (fp2mul (r0_228) (r0_228))
+  in
+  let a_231 :=
+    fp2mul (a_230) (
+      fp2inv (
+        fp2mul (
+          fp2fromfp (
+            nat_two )) (
+          r1_229)))
+  in
+  let b_232 := fp2sub (r1_229) (fp2mul (a_231) (r0_228)) in
+  let a_233 := fp12fromfp6 (fp6fromfp2 (a_231)) in
+  let b_234 := fp12fromfp6 (fp6fromfp2 (b_232)) in
+  let '(x_235, y_236) := twist (p_227) in
+  fp12neg (fp12sub (fp12sub (y_236) (fp12mul (a_233) (x_235))) (b_234)).
+
+Definition line_add_p (r_237 : g2) (q_238 : g2) (p_239 : g1) : fp12 :=
+  let '(r0_240, r1_241, _) := r_237 in
+  let '(q0_242, q1_243, _) := q_238 in
+  let a_244 :=
+    fp2mul (fp2sub (q1_243) (r1_241)) (fp2inv (fp2sub (q0_242) (r0_240)))
+  in
+  let b_245 := fp2sub (r1_241) (fp2mul (a_244) (r0_240)) in
+  let a_246 := fp12fromfp6 (fp6fromfp2 (a_244)) in
+  let b_247 := fp12fromfp6 (fp6fromfp2 (b_245)) in
+  let '(x_248, y_249) := twist (p_239) in
+  fp12neg (fp12sub (fp12sub (y_249) (fp12mul (a_246) (x_248))) (b_247)).
+
+(* TODO *)
+Axiom array_to_le_bytes : forall {l}, lseq N l  -> int.
+
+Definition frobenius (f_250 : fp12) : fp12 :=
+  let '((g0_251, g1_252, g2_253), (h0_254, h1_255, h2_256)) := f_250 in
+  let t1_257 := fp2conjugate (g0_251) in
+  let t2_258 := fp2conjugate (h0_254) in
+  let t3_259 := fp2conjugate (g1_252) in
+  let t4_260 := fp2conjugate (h1_255) in
+  let t5_261 := fp2conjugate (g2_253) in
+  let t6_262 := fp2conjugate (h2_256) in
+  let c1_263 :=
+    array_from_list (
+      let l :=
+        [
+          secret (pub_u64 10162220747404304312);
+          secret (pub_u64 17761815663483519293);
+          secret (pub_u64 8873291758750579140);
+          secret (pub_u64 1141103941765652303);
+          secret (pub_u64 13993175198059990303);
+          secret (pub_u64 1802798568193066599)
+        ]
+      in l)
+  in
+  let c1_264 := array_to_le_bytes (c1_263) in
+  let c1_265 := c1_264 in
+  let c2_266 :=
+    array_from_list (
+      let l :=
+        [
+          secret (pub_u64 3240210268673559283);
+          secret (pub_u64 2895069921743240898);
+          secret (pub_u64 17009126888523054175);
+          secret (pub_u64 6098234018649060207);
+          secret (pub_u64 9865672654120263608);
+          secret (pub_u64 71000049454473266)
+        ]
+      in l)
+  in
+  let c2_267 := array_to_le_bytes (c2_266) in
+  let c2_268 := c2_267
+  in
+  let gamma11_269 := (c1_265, c2_268) in
+  let gamma12_270 := fp2mul (gamma11_269) (gamma11_269) in
+  let gamma13_271 := fp2mul (gamma12_270) (gamma11_269) in
+  let gamma14_272 := fp2mul (gamma13_271) (gamma11_269) in
+  let gamma15_273 := fp2mul (gamma14_272) (gamma11_269) in
+  let t2_274 := fp2mul (t2_258) (gamma11_269) in
+  let t3_275 := fp2mul (t3_259) (gamma12_270) in
+  let t4_276 := fp2mul (t4_260) (gamma13_271) in
+  let t5_277 := fp2mul (t5_261) (gamma14_272) in
+  let t6_278 := fp2mul (t6_262) (gamma15_273) in
+  ((t1_257, t3_275, t5_277), (t2_274, t4_276, t6_278)).
+
+Import nat_mod_0x8000000000000000000000000000000000000000000000000000000000000000.
+Infix "/" := divs.
+
+Definition final_exponentiation (f_279 : fp12) : fp12 :=
+  let fp6_280 := fp12conjugate (f_279) in
+  let finv_281 := fp12inv (f_279) in
+  let fp6_1_282 := fp12mul (fp6_280) (finv_281) in
+  let fp8_283 := frobenius (frobenius (fp6_1_282)) in
+  let f_284 := fp12mul (fp8_283) (fp6_1_282) in
+  let u_285 :=
+    repr (
+      pub_u128 15132376222941642752)
+  in
+  let t0_286 := fp12mul (f_284) (f_284) in
+  let t1_287 := fp12exp (t0_286) (u_285) in
+  let t1_288 := fp12conjugate (t1_287) in
+  let t2_289 :=
+    fp12exp (t1_288) (
+      (u_285) / (
+        (repr 2)))
+  in
+  let t2_290 := fp12conjugate (t2_289) in
+  let t3_291 := fp12conjugate (f_284) in
+  let t1_292 := fp12mul (t3_291) (t1_288) in
+  let t1_293 := fp12conjugate (t1_292) in
+  let t1_294 := fp12mul (t1_293) (t2_290) in
+  let t2_295 := fp12exp (t1_294) (u_285) in
+  let t2_296 := fp12conjugate (t2_295) in
+  let t3_297 := fp12exp (t2_296) (u_285) in
+  let t3_298 := fp12conjugate (t3_297) in
+  let t1_299 := fp12conjugate (t1_294) in
+  let t3_300 := fp12mul (t1_299) (t3_298) in
+  let t1_301 := fp12conjugate (t1_299) in
+  let t1_302 := frobenius (frobenius (frobenius (t1_301))) in
+  let t2_303 := frobenius (frobenius (t2_296)) in
+  let t1_304 := fp12mul (t1_302) (t2_303) in
+  let t2_305 := fp12exp (t3_300) (u_285) in
+  let t2_306 := fp12conjugate (t2_305) in
+  let t2_307 := fp12mul (t2_306) (t0_286) in
+  let t2_308 := fp12mul (t2_307) (f_284) in
+  let t1_309 := fp12mul (t1_304) (t2_308) in
+  let t2_310 := frobenius (t3_300) in
+  let t1_311 := fp12mul (t1_309) (t2_310) in
+  t1_311.
+
+Definition pairing (p_312 : g1) (q_313 : g2) : fp12 :=
+  let t_314 :=
+    repr (
+      pub_u128 15132376222941642752)
+  in
+  let r_315 := q_313 in
+  let f_316 :=
+    fp12fromfp6 (
+      fp6fromfp2 (
+        fp2fromfp (
+          nat_one)))
+  in
+  let '(r_315, f_316) :=
+    foldi (usize 1) (usize 64) (fun i_317 '(r_315, f_316) =>
+      let lrr_318 := line_double_p (r_315) (p_312) in
+      let r_315 := g2double (r_315) in
+      let f_316 := fp12mul (fp12mul (f_316) (f_316)) (lrr_318) in
+      let (r_315, f_316) :=
+        if nat_bit (0x8000000000000000000000000000000000000000000000000000000000000000) (
+          t_314) (((usize 64) - (i_317)) - (usize 1)) then (
+          let lrq_319 := line_add_p (r_315) (q_313) (p_312) in
+          let r_315 := g2add (r_315) (q_313) in
+          let f_316 := fp12mul (f_316) (lrq_319) in
+          (r_315, f_316)
+        ) else ( (r_315, f_316)
+        )
+      in
+      (r_315, f_316))
+    (r_315, f_316)
+  in
+  final_exponentiation (fp12conjugate (f_316)).
+
